fairness/lawyer/obligations/wf_utils.v
@@ -1,0 +1,19 @@
+Require Import Coq.Program.Wf.
+From stdpp Require Import relations.
+
+
+Section WfSetMin.
+  Context {A: Type}.
+
+  Definition minimal_in_prop (R : relation A) (x : A) (P : A -> Prop) :=
+    forall y, P y -> R y x -> R x y. 
+  
+  Context {R: relation A}.
+  Hypothesis (WF: wf R).
+
+  Theorem sets_have_min (P: A -> Prop)
+    (NE: exists a, P a):
+    exists a, P a /\ minimal_in_prop R a P.
+  Proof. Admitted.
+  
+End WfSetMin.
